<?xml version="1.0"?>
<rdf:RDF xmlns="http://purl.obolibrary.org/obo/occo/dev/skill_types.owl#"
     xml:base="http://purl.obolibrary.org/obo/occo/dev/skill_types.owl"
     xmlns:obo="http://purl.obolibrary.org/obo/"
     xmlns:owl="http://www.w3.org/2002/07/owl#"
     xmlns:rdf="http://www.w3.org/1999/02/22-rdf-syntax-ns#"
     xmlns:xml="http://www.w3.org/XML/1998/namespace"
     xmlns:xsd="http://www.w3.org/2001/XMLSchema#"
     xmlns:rdfs="http://www.w3.org/2000/01/rdf-schema#">
    <owl:Ontology rdf:about="http://purl.obolibrary.org/obo/occo/dev/skill_types.owl"/>
    


    <!-- 
    ///////////////////////////////////////////////////////////////////////////////////////
    //
    // Annotation properties
    //
    ///////////////////////////////////////////////////////////////////////////////////////
     -->

    


    <!-- http://purl.obolibrary.org/obo/IAO_0000115 -->

    <owl:AnnotationProperty rdf:about="http://purl.obolibrary.org/obo/IAO_0000115"/>
    


    <!-- http://purl.obolibrary.org/obo/IAO_0000117 -->

    <owl:AnnotationProperty rdf:about="http://purl.obolibrary.org/obo/IAO_0000117"/>
    


    <!-- http://purl.obolibrary.org/obo/IAO_0000119 -->

    <owl:AnnotationProperty rdf:about="http://purl.obolibrary.org/obo/IAO_0000119"/>
    


    <!-- http://purl.obolibrary.org/obo/OCCO_00000008 -->

    <owl:AnnotationProperty rdf:about="http://purl.obolibrary.org/obo/OCCO_00000008"/>
    


    <!-- 
    ///////////////////////////////////////////////////////////////////////////////////////
    //
    // Classes
    //
    ///////////////////////////////////////////////////////////////////////////////////////
     -->

    


    <!-- http://purl.obolibrary.org/obo/OCCO_00000003 -->

    <owl:Class rdf:about="http://purl.obolibrary.org/obo/OCCO_00000003"/>
    


    <!-- http://purl.obolibrary.org/obo/OCCO_00000020 -->

    <owl:Class rdf:about="http://purl.obolibrary.org/obo/OCCO_00000020">
        <rdfs:subClassOf rdf:resource="http://purl.obolibrary.org/obo/OCCO_00000003"/>
        <obo:IAO_0000115>A skill realized in understanding the implications of new information for both current and future problem-solving and decision-making.</obo:IAO_0000115>
        <obo:IAO_0000117>Oliver He</obo:IAO_0000117>
        <obo:IAO_0000117>Sam Smith</obo:IAO_0000117>
        <obo:IAO_0000119>https://www.onetonline.org/skills/soft/</obo:IAO_0000119>
        <obo:OCCO_00000008>2.A.2.b</obo:OCCO_00000008>
        <rdfs:label>active learning</rdfs:label>
    </owl:Class>
    


    <!-- http://purl.obolibrary.org/obo/OCCO_00000021 -->

    <owl:Class rdf:about="http://purl.obolibrary.org/obo/OCCO_00000021">
        <rdfs:subClassOf rdf:resource="http://purl.obolibrary.org/obo/OCCO_00000003"/>
        <obo:IAO_0000115>A skill realized in giving full attention to what other people are saying, taking time to understand the points being made, asking questions as appropriate, and not interrupting at inappropriate times.</obo:IAO_0000115>
        <obo:IAO_0000117>Oliver He</obo:IAO_0000117>
        <obo:IAO_0000117>Sam Smith</obo:IAO_0000117>
        <obo:IAO_0000119>https://www.onetonline.org/skills/soft/</obo:IAO_0000119>
        <obo:OCCO_00000008>2.A.1.b</obo:OCCO_00000008>
        <rdfs:label>active listening</rdfs:label>
    </owl:Class>
    


    <!-- http://purl.obolibrary.org/obo/OCCO_00000022 -->

    <owl:Class rdf:about="http://purl.obolibrary.org/obo/OCCO_00000022">
        <rdfs:subClassOf rdf:resource="http://purl.obolibrary.org/obo/OCCO_00000003"/>
        <obo:IAO_0000115>A skill realized in identifying complex problems and reviewing related information to develop and evaluate options and implement solutions.</obo:IAO_0000115>
        <obo:IAO_0000117>Oliver He</obo:IAO_0000117>
        <obo:IAO_0000117>Sam Smith</obo:IAO_0000117>
        <obo:IAO_0000119>https://www.onetonline.org/skills/soft/</obo:IAO_0000119>
        <obo:OCCO_00000008>2.B.2.i</obo:OCCO_00000008>
        <rdfs:label>complex problem solving</rdfs:label>
    </owl:Class>
    


    <!-- http://purl.obolibrary.org/obo/OCCO_00000023 -->

    <owl:Class rdf:about="http://purl.obolibrary.org/obo/OCCO_00000023">
        <rdfs:subClassOf rdf:resource="http://purl.obolibrary.org/obo/OCCO_00000003"/>
        <obo:IAO_0000115>A skill realized in adjusting actions in relation to others&apos; actions.</obo:IAO_0000115>
        <obo:IAO_0000117>Oliver He</obo:IAO_0000117>
        <obo:IAO_0000117>Sam Smith</obo:IAO_0000117>
        <obo:IAO_0000119>https://www.onetonline.org/find/descriptor/browse/2.B/2.B.2/2.B.5/2.B.1/2.B.4/2.B.3</obo:IAO_0000119>
        <obo:OCCO_00000008>2.B.1.b</obo:OCCO_00000008>
        <rdfs:label>coordination</rdfs:label>
    </owl:Class>
    


    <!-- http://purl.obolibrary.org/obo/OCCO_00000024 -->

    <owl:Class rdf:about="http://purl.obolibrary.org/obo/OCCO_00000024">
        <rdfs:subClassOf rdf:resource="http://purl.obolibrary.org/obo/OCCO_00000003"/>
        <obo:IAO_0000115>A skill realized in using logic and reasoning to identify the strengths and weaknesses of alternative solutions, conclusions or approaches to problems.</obo:IAO_0000115>
        <obo:IAO_0000117>Oliver He</obo:IAO_0000117>
        <obo:IAO_0000117>Sam Smith</obo:IAO_0000117>
        <obo:IAO_0000119>https://www.onetonline.org/skills/soft/</obo:IAO_0000119>
        <obo:OCCO_00000008>2.A.2.a</obo:OCCO_00000008>
        <rdfs:label>critical thinking</rdfs:label>
    </owl:Class>
    


    <!-- http://purl.obolibrary.org/obo/OCCO_00000025 -->

    <owl:Class rdf:about="http://purl.obolibrary.org/obo/OCCO_00000025">
        <rdfs:subClassOf rdf:resource="http://purl.obolibrary.org/obo/OCCO_00000003"/>
        <obo:IAO_0000115>A skill realized in performing routine maintenance on equipment and determining when and what kind of maintenance is needed.</obo:IAO_0000115>
        <obo:IAO_0000117>Oliver He</obo:IAO_0000117>
        <obo:IAO_0000117>Sam Smith</obo:IAO_0000117>
        <obo:IAO_0000119>https://www.onetonline.org/find/descriptor/browse/2.B/2.B.2/2.B.5/2.B.1/2.B.4/2.B.3</obo:IAO_0000119>
        <obo:OCCO_00000008>2.B.3.j</obo:OCCO_00000008>
        <rdfs:label>equipment maintenance</rdfs:label>
    </owl:Class>
    


    <!-- http://purl.obolibrary.org/obo/OCCO_00000026 -->

    <owl:Class rdf:about="http://purl.obolibrary.org/obo/OCCO_00000026">
        <rdfs:subClassOf rdf:resource="http://purl.obolibrary.org/obo/OCCO_00000003"/>
        <obo:IAO_0000115>A skill realized in determining the kind of tools and equipment needed to do a job.</obo:IAO_0000115>
        <obo:IAO_0000117>Oliver He</obo:IAO_0000117>
        <obo:IAO_0000117>Sam Smith</obo:IAO_0000117>
        <obo:IAO_0000119>https://www.onetonline.org/find/descriptor/browse/2.B/2.B.2/2.B.5/2.B.1/2.B.4/2.B.3</obo:IAO_0000119>
        <obo:OCCO_00000008>2.B.3.c</obo:OCCO_00000008>
        <rdfs:label>equipment selection</rdfs:label>
    </owl:Class>
    


    <!-- http://purl.obolibrary.org/obo/OCCO_00000027 -->

    <owl:Class rdf:about="http://purl.obolibrary.org/obo/OCCO_00000027">
        <rdfs:subClassOf rdf:resource="http://purl.obolibrary.org/obo/OCCO_00000003"/>
        <obo:IAO_0000115>A skill realized in installing equipment, machines, wiring, or programs to meet specifications.</obo:IAO_0000115>
        <obo:IAO_0000117>Oliver He</obo:IAO_0000117>
        <obo:IAO_0000117>Sam Smith</obo:IAO_0000117>
        <obo:IAO_0000119>https://www.onetonline.org/find/descriptor/browse/2.B/2.B.2/2.B.5/2.B.1/2.B.4/2.B.3</obo:IAO_0000119>
        <obo:OCCO_00000008>2.B.3.d</obo:OCCO_00000008>
        <rdfs:label>installation</rdfs:label>
    </owl:Class>
    


    <!-- http://purl.obolibrary.org/obo/OCCO_00000028 -->

    <owl:Class rdf:about="http://purl.obolibrary.org/obo/OCCO_00000028">
        <rdfs:subClassOf rdf:resource="http://purl.obolibrary.org/obo/OCCO_00000003"/>
        <obo:IAO_0000115>A skill realized in teaching others how to do something.</obo:IAO_0000115>
        <obo:IAO_0000117>Oliver He</obo:IAO_0000117>
        <obo:IAO_0000117>Sam Smith</obo:IAO_0000117>
        <obo:IAO_0000119>https://www.onetonline.org/skills/soft/</obo:IAO_0000119>
        <obo:OCCO_00000008>2.B.1.e</obo:OCCO_00000008>
        <rdfs:label>instructing</rdfs:label>
    </owl:Class>
    


    <!-- http://purl.obolibrary.org/obo/OCCO_00000029 -->

    <owl:Class rdf:about="http://purl.obolibrary.org/obo/OCCO_00000029">
        <rdfs:subClassOf rdf:resource="http://purl.obolibrary.org/obo/OCCO_00000003"/>
        <obo:IAO_0000115>A skill realized in considering the relative costs and benefits of potential actions to choose the most appropriate one.</obo:IAO_0000115>
        <obo:IAO_0000117>Oliver He</obo:IAO_0000117>
        <obo:IAO_0000117>Sam Smith</obo:IAO_0000117>
        <obo:IAO_0000119>https://www.onetonline.org/find/descriptor/browse/2.B/2.B.2/2.B.5/2.B.1/2.B.4/2.B.3</obo:IAO_0000119>
        <obo:OCCO_00000008>2.B.4.e</obo:OCCO_00000008>
        <rdfs:label>judgment and decision making</rdfs:label>
    </owl:Class>
    


    <!-- http://purl.obolibrary.org/obo/OCCO_00000030 -->

    <owl:Class rdf:about="http://purl.obolibrary.org/obo/OCCO_00000030">
        <rdfs:subClassOf rdf:resource="http://purl.obolibrary.org/obo/OCCO_00000003"/>
        <obo:IAO_0000115>A skill realized in selecting and using training/instructional methods and procedures appropriate for the situation when learning or teaching new things.</obo:IAO_0000115>
        <obo:IAO_0000117>Oliver He</obo:IAO_0000117>
        <obo:IAO_0000117>Sam Smith</obo:IAO_0000117>
        <obo:IAO_0000119>https://www.onetonline.org/skills/soft/</obo:IAO_0000119>
        <obo:OCCO_00000008>2.A.2.c</obo:OCCO_00000008>
        <rdfs:label>learning strategies</rdfs:label>
    </owl:Class>
    


    <!-- http://purl.obolibrary.org/obo/OCCO_00000031 -->

    <owl:Class rdf:about="http://purl.obolibrary.org/obo/OCCO_00000031">
        <rdfs:subClassOf rdf:resource="http://purl.obolibrary.org/obo/OCCO_00000003"/>
        <obo:IAO_0000115>A skill realized in determining how money will be spent to get the work done, and accounting for these expenditures.</obo:IAO_0000115>
        <obo:IAO_0000117>Oliver He</obo:IAO_0000117>
        <obo:IAO_0000117>Sam Smith</obo:IAO_0000117>
        <obo:IAO_0000119>https://www.onetonline.org/find/descriptor/browse/2.B/2.B.2/2.B.5/2.B.1/2.B.4/2.B.3</obo:IAO_0000119>
        <obo:OCCO_00000008>2.B.5.b</obo:OCCO_00000008>
        <rdfs:label>management of financial resources</rdfs:label>
    </owl:Class>
    


    <!-- http://purl.obolibrary.org/obo/OCCO_00000032 -->

    <owl:Class rdf:about="http://purl.obolibrary.org/obo/OCCO_00000032">
        <rdfs:subClassOf rdf:resource="http://purl.obolibrary.org/obo/OCCO_00000003"/>
        <obo:IAO_0000115>A skill realized in obtaining and seeing to the appropriate use of equipment, facilities, and materials needed to do certain work.</obo:IAO_0000115>
        <obo:IAO_0000117>Oliver He</obo:IAO_0000117>
        <obo:IAO_0000117>Sam Smith</obo:IAO_0000117>
        <obo:IAO_0000119>https://www.onetonline.org/find/descriptor/browse/2.B/2.B.2/2.B.5/2.B.1/2.B.4/2.B.3</obo:IAO_0000119>
        <obo:OCCO_00000008>2.B.5.c</obo:OCCO_00000008>
        <rdfs:label>management of material resources</rdfs:label>
    </owl:Class>
    


    <!-- http://purl.obolibrary.org/obo/OCCO_00000033 -->

    <owl:Class rdf:about="http://purl.obolibrary.org/obo/OCCO_00000033">
        <rdfs:subClassOf rdf:resource="http://purl.obolibrary.org/obo/OCCO_00000003"/>
        <obo:IAO_0000115>A skill realized in motivating, developing, and directing people as they work, identifying the best people for the job.</obo:IAO_0000115>
        <obo:IAO_0000117>Oliver He</obo:IAO_0000117>
        <obo:IAO_0000117>Sam Smith</obo:IAO_0000117>
        <obo:IAO_0000119>https://www.onetonline.org/find/descriptor/browse/2.B/2.B.2/2.B.5/2.B.1/2.B.4/2.B.3</obo:IAO_0000119>
        <obo:OCCO_00000008>2.B.5.d</obo:OCCO_00000008>
        <rdfs:label>management of personnel resources</rdfs:label>
    </owl:Class>
    


    <!-- http://purl.obolibrary.org/obo/OCCO_00000034 -->

    <owl:Class rdf:about="http://purl.obolibrary.org/obo/OCCO_00000034">
        <rdfs:subClassOf rdf:resource="http://purl.obolibrary.org/obo/OCCO_00000003"/>
        <obo:IAO_0000115>A skill realized in using mathematics to solve problems.</obo:IAO_0000115>
        <obo:IAO_0000117>Oliver He</obo:IAO_0000117>
        <obo:IAO_0000117>Sam Smith</obo:IAO_0000117>
        <obo:IAO_0000119>https://www.onetonline.org/find/descriptor/browse/2.A/2.A.1/2.A.2</obo:IAO_0000119>
        <obo:OCCO_00000008>2.A.1.e</obo:OCCO_00000008>
        <rdfs:label>mathematics</rdfs:label>
    </owl:Class>
    


    <!-- http://purl.obolibrary.org/obo/OCCO_00000035 -->

    <owl:Class rdf:about="http://purl.obolibrary.org/obo/OCCO_00000035">
        <rdfs:subClassOf rdf:resource="http://purl.obolibrary.org/obo/OCCO_00000003"/>
        <obo:IAO_0000115>A skill realized in monitoring/Assessing performance of yourself, other individuals, or organizations to make improvements or take corrective action.</obo:IAO_0000115>
        <obo:IAO_0000117>Oliver He</obo:IAO_0000117>
        <obo:IAO_0000117>Sam Smith</obo:IAO_0000117>
        <obo:IAO_0000119>https://www.onetonline.org/skills/soft/</obo:IAO_0000119>
        <obo:OCCO_00000008>2.A.2.d</obo:OCCO_00000008>
        <rdfs:label>monitoring</rdfs:label>
    </owl:Class>
    


    <!-- http://purl.obolibrary.org/obo/OCCO_00000036 -->

    <owl:Class rdf:about="http://purl.obolibrary.org/obo/OCCO_00000036">
        <rdfs:subClassOf rdf:resource="http://purl.obolibrary.org/obo/OCCO_00000003"/>
        <obo:IAO_0000115>A skill realized in bringing others together and trying to reconcile differences.</obo:IAO_0000115>
        <obo:IAO_0000117>Oliver He</obo:IAO_0000117>
        <obo:IAO_0000117>Sam Smith</obo:IAO_0000117>
        <obo:IAO_0000119>https://www.onetonline.org/skills/soft/</obo:IAO_0000119>
        <obo:OCCO_00000008>2.B.1.d</obo:OCCO_00000008>
        <rdfs:label>negotiation</rdfs:label>
    </owl:Class>
    


    <!-- http://purl.obolibrary.org/obo/OCCO_00000037 -->

    <owl:Class rdf:about="http://purl.obolibrary.org/obo/OCCO_00000037">
        <rdfs:subClassOf rdf:resource="http://purl.obolibrary.org/obo/OCCO_00000003"/>
        <obo:IAO_0000115>A skill realized in controlling operations of equipment or systems.</obo:IAO_0000115>
        <obo:IAO_0000117>Oliver He</obo:IAO_0000117>
        <obo:IAO_0000117>Sam Smith</obo:IAO_0000117>
        <obo:IAO_0000119>https://www.onetonline.org/find/descriptor/browse/2.B/2.B.2/2.B.5/2.B.1/2.B.4/2.B.3</obo:IAO_0000119>
        <obo:OCCO_00000008>2.B.3.h</obo:OCCO_00000008>
        <rdfs:label>operation and control</rdfs:label>
    </owl:Class>
    


    <!-- http://purl.obolibrary.org/obo/OCCO_00000038 -->

    <owl:Class rdf:about="http://purl.obolibrary.org/obo/OCCO_00000038">
        <rdfs:subClassOf rdf:resource="http://purl.obolibrary.org/obo/OCCO_00000003"/>
        <obo:IAO_0000115>A skill realized in matching gauges, dials, or other indicators to make sure a machine is working properly.</obo:IAO_0000115>
        <obo:IAO_0000117>Oliver He</obo:IAO_0000117>
        <obo:IAO_0000117>Sam Smith</obo:IAO_0000117>
        <obo:IAO_0000119>https://www.onetonline.org/find/descriptor/browse/2.B/2.B.2/2.B.5/2.B.1/2.B.4/2.B.3</obo:IAO_0000119>
        <obo:OCCO_00000008>2.B.3.g</obo:OCCO_00000008>
        <rdfs:label>operation monitoring</rdfs:label>
    </owl:Class>
    


    <!-- http://purl.obolibrary.org/obo/OCCO_00000039 -->

    <owl:Class rdf:about="http://purl.obolibrary.org/obo/OCCO_00000039">
        <rdfs:subClassOf rdf:resource="http://purl.obolibrary.org/obo/OCCO_00000003"/>
        <obo:IAO_0000115>A skill realized in analyzing needs and product requirements to create a design.</obo:IAO_0000115>
        <obo:IAO_0000117>Oliver He</obo:IAO_0000117>
        <obo:IAO_0000117>Sam Smith</obo:IAO_0000117>
        <obo:IAO_0000119>https://www.onetonline.org/find/descriptor/browse/2.B/2.B.2/2.B.5/2.B.1/2.B.4/2.B.3</obo:IAO_0000119>
        <obo:OCCO_00000008>2.B.3.a</obo:OCCO_00000008>
        <rdfs:label>operations analysis</rdfs:label>
    </owl:Class>
    


    <!-- http://purl.obolibrary.org/obo/OCCO_00000040 -->

    <owl:Class rdf:about="http://purl.obolibrary.org/obo/OCCO_00000040">
        <rdfs:subClassOf rdf:resource="http://purl.obolibrary.org/obo/OCCO_00000003"/>
        <obo:IAO_0000115>A skill realized in persuading others to change their minds or behavior.</obo:IAO_0000115>
        <obo:IAO_0000117>Oliver He</obo:IAO_0000117>
        <obo:IAO_0000117>Sam Smith</obo:IAO_0000117>
        <obo:IAO_0000119>https://www.onetonline.org/find/descriptor/browse/2.B/2.B.2/2.B.5/2.B.1/2.B.4/2.B.3</obo:IAO_0000119>
        <obo:OCCO_00000008>2.B.1.c</obo:OCCO_00000008>
        <rdfs:label>persuasion</rdfs:label>
    </owl:Class>
    


    <!-- http://purl.obolibrary.org/obo/OCCO_00000041 -->

    <owl:Class rdf:about="http://purl.obolibrary.org/obo/OCCO_00000041">
        <rdfs:subClassOf rdf:resource="http://purl.obolibrary.org/obo/OCCO_00000003"/>
        <obo:IAO_0000115>A skill realized in writing computer programs for various purposes.</obo:IAO_0000115>
        <obo:IAO_0000117>Oliver He</obo:IAO_0000117>
        <obo:IAO_0000117>Sam Smith</obo:IAO_0000117>
        <obo:IAO_0000119>https://www.onetonline.org/find/descriptor/browse/2.B/2.B.2/2.B.5/2.B.1/2.B.4/2.B.3</obo:IAO_0000119>
        <obo:OCCO_00000008>2.B.3.e</obo:OCCO_00000008>
        <rdfs:label>programming</rdfs:label>
    </owl:Class>
    


    <!-- http://purl.obolibrary.org/obo/OCCO_00000042 -->

    <owl:Class rdf:about="http://purl.obolibrary.org/obo/OCCO_00000042">
        <rdfs:subClassOf rdf:resource="http://purl.obolibrary.org/obo/OCCO_00000003"/>
        <obo:IAO_0000115>A skill realized in conducting tests and inspections of products, services, or processes to evaluate quality or performance.</obo:IAO_0000115>
        <obo:IAO_0000117>Oliver He</obo:IAO_0000117>
        <obo:IAO_0000117>Sam Smith</obo:IAO_0000117>
        <obo:IAO_0000119>https://www.onetonline.org/find/descriptor/browse/2.B/2.B.2/2.B.5/2.B.1/2.B.4/2.B.3</obo:IAO_0000119>
        <obo:OCCO_00000008>2.B.3.m</obo:OCCO_00000008>
        <rdfs:label>quality control analysis</rdfs:label>
    </owl:Class>
    


    <!-- http://purl.obolibrary.org/obo/OCCO_00000043 -->

    <owl:Class rdf:about="http://purl.obolibrary.org/obo/OCCO_00000043">
        <rdfs:subClassOf rdf:resource="http://purl.obolibrary.org/obo/OCCO_00000003"/>
        <obo:IAO_0000115>A skill realized in understanding written sentences and paragraphs in work related documents.</obo:IAO_0000115>
        <obo:IAO_0000117>Oliver He</obo:IAO_0000117>
        <obo:IAO_0000117>Sam Smith</obo:IAO_0000117>
        <obo:IAO_0000119>https://www.onetonline.org/find/descriptor/browse/2.A/2.A.1/2.A.2</obo:IAO_0000119>
        <obo:OCCO_00000008>2.A.1.a</obo:OCCO_00000008>
        <rdfs:label>reading comprehension</rdfs:label>
    </owl:Class>
    


    <!-- http://purl.obolibrary.org/obo/OCCO_00000044 -->

    <owl:Class rdf:about="http://purl.obolibrary.org/obo/OCCO_00000044">
        <rdfs:subClassOf rdf:resource="http://purl.obolibrary.org/obo/OCCO_00000003"/>
        <obo:IAO_0000115>A skill realized in repairing machines or systems using the needed tools.</obo:IAO_0000115>
        <obo:IAO_0000117>Oliver He</obo:IAO_0000117>
        <obo:IAO_0000117>Sam Smith</obo:IAO_0000117>
        <obo:IAO_0000119>https://www.onetonline.org/find/descriptor/browse/2.B/2.B.2/2.B.5/2.B.1/2.B.4/2.B.3</obo:IAO_0000119>
        <obo:OCCO_00000008>2.B.3.l</obo:OCCO_00000008>
        <rdfs:label>repairing</rdfs:label>
    </owl:Class>
    


    <!-- http://purl.obolibrary.org/obo/OCCO_00000045 -->

    <owl:Class rdf:about="http://purl.obolibrary.org/obo/OCCO_00000045">
        <rdfs:subClassOf rdf:resource="http://purl.obolibrary.org/obo/OCCO_00000003"/>
        <obo:IAO_0000115>A skill realized in using scientific rules and methods to solve problems.</obo:IAO_0000115>
        <obo:IAO_0000117>Oliver He</obo:IAO_0000117>
        <obo:IAO_0000117>Sam Smith</obo:IAO_0000117>
        <obo:IAO_0000119>https://www.onetonline.org/find/descriptor/browse/2.A/2.A.1/2.A.2</obo:IAO_0000119>
        <obo:OCCO_00000008>2.A.1.f</obo:OCCO_00000008>
        <rdfs:label>science</rdfs:label>
    </owl:Class>
    


    <!-- http://purl.obolibrary.org/obo/OCCO_00000046 -->

    <owl:Class rdf:about="http://purl.obolibrary.org/obo/OCCO_00000046">
        <rdfs:subClassOf rdf:resource="http://purl.obolibrary.org/obo/OCCO_00000003"/>
        <obo:IAO_0000115>A skill realized in actively looking for ways to help people.</obo:IAO_0000115>
        <obo:IAO_0000117>Oliver He</obo:IAO_0000117>
        <obo:IAO_0000117>Sam Smith</obo:IAO_0000117>
        <obo:IAO_0000119>https://www.onetonline.org/skills/soft/</obo:IAO_0000119>
        <obo:OCCO_00000008>2.B.1.f</obo:OCCO_00000008>
        <rdfs:label>service orientation</rdfs:label>
    </owl:Class>
    


    <!-- http://purl.obolibrary.org/obo/OCCO_00000047 -->

    <owl:Class rdf:about="http://purl.obolibrary.org/obo/OCCO_00000047">
        <rdfs:subClassOf rdf:resource="http://purl.obolibrary.org/obo/OCCO_00000003"/>
        <obo:IAO_0000115>A skill realized in being aware of others&apos; reactions and understanding why they react as they do.</obo:IAO_0000115>
        <obo:IAO_0000117>Oliver He</obo:IAO_0000117>
        <obo:IAO_0000117>Sam Smith</obo:IAO_0000117>
        <obo:IAO_0000119>https://www.onetonline.org/find/descriptor/browse/2.B/2.B.2/2.B.5/2.B.1/2.B.4/2.B.3</obo:IAO_0000119>
        <obo:OCCO_00000008>2.B.1.a</obo:OCCO_00000008>
        <rdfs:label>social perceptiveness</rdfs:label>
    </owl:Class>
    


    <!-- http://purl.obolibrary.org/obo/OCCO_00000048 -->

    <owl:Class rdf:about="http://purl.obolibrary.org/obo/OCCO_00000048">
        <rdfs:subClassOf rdf:resource="http://purl.obolibrary.org/obo/OCCO_00000003"/>
        <obo:IAO_0000115>A skill realized in talking to others to convey information effectively.</obo:IAO_0000115>
        <obo:IAO_0000117>Oliver He</obo:IAO_0000117>
        <obo:IAO_0000117>Sam Smith</obo:IAO_0000117>
        <obo:IAO_0000119>https://www.onetonline.org/find/descriptor/browse/2.A/2.A.1/2.A.2</obo:IAO_0000119>
        <obo:OCCO_00000008>2.A.1.d</obo:OCCO_00000008>
        <rdfs:label>speaking</rdfs:label>
    </owl:Class>
    


    <!-- http://purl.obolibrary.org/obo/OCCO_00000049 -->

    <owl:Class rdf:about="http://purl.obolibrary.org/obo/OCCO_00000049">
        <rdfs:subClassOf rdf:resource="http://purl.obolibrary.org/obo/OCCO_00000003"/>
        <obo:IAO_0000115>A skill realized in determining how a system should work and how changes in conditions, operations, and the environment will affect outcomes.</obo:IAO_0000115>
        <obo:IAO_0000117>Oliver He</obo:IAO_0000117>
        <obo:IAO_0000117>Sam Smith</obo:IAO_0000117>
        <obo:IAO_0000119>https://www.onetonline.org/find/descriptor/browse/2.B/2.B.2/2.B.5/2.B.1/2.B.4/2.B.3</obo:IAO_0000119>
        <obo:OCCO_00000008>2.B.4.g</obo:OCCO_00000008>
        <rdfs:label>systems analysis</rdfs:label>
    </owl:Class>
    


    <!-- http://purl.obolibrary.org/obo/OCCO_00000050 -->

    <owl:Class rdf:about="http://purl.obolibrary.org/obo/OCCO_00000050">
        <rdfs:subClassOf rdf:resource="http://purl.obolibrary.org/obo/OCCO_00000003"/>
        <obo:IAO_0000115>A skill realized in identifying measures or indicators of system performance and the actions needed to improve or correct performance, relative to the goals of the system.</obo:IAO_0000115>
        <obo:IAO_0000117>Oliver He</obo:IAO_0000117>
        <obo:IAO_0000117>Sam Smith</obo:IAO_0000117>
        <obo:IAO_0000119>https://www.onetonline.org/find/descriptor/browse/2.B/2.B.2/2.B.5/2.B.1/2.B.4/2.B.3</obo:IAO_0000119>
        <obo:OCCO_00000008>2.B.4.h</obo:OCCO_00000008>
        <rdfs:label>systems evaluation</rdfs:label>
    </owl:Class>
    


    <!-- http://purl.obolibrary.org/obo/OCCO_00000051 -->

    <owl:Class rdf:about="http://purl.obolibrary.org/obo/OCCO_00000051">
        <rdfs:subClassOf rdf:resource="http://purl.obolibrary.org/obo/OCCO_00000003"/>
        <obo:IAO_0000115>A skill realized in generating or adapting equipment and technology to serve user needs.</obo:IAO_0000115>
        <obo:IAO_0000117>Oliver He</obo:IAO_0000117>
        <obo:IAO_0000117>Sam Smith</obo:IAO_0000117>
        <obo:IAO_0000119>https://www.onetonline.org/find/descriptor/browse/2.B/2.B.2/2.B.5/2.B.1/2.B.4/2.B.3</obo:IAO_0000119>
        <obo:OCCO_00000008>2.B.3.b</obo:OCCO_00000008>
        <rdfs:label>technology design</rdfs:label>
    </owl:Class>
    


    <!-- http://purl.obolibrary.org/obo/OCCO_00000052 -->

    <owl:Class rdf:about="http://purl.obolibrary.org/obo/OCCO_00000052">
        <rdfs:subClassOf rdf:resource="http://purl.obolibrary.org/obo/OCCO_00000003"/>
        <obo:IAO_0000115>A skill realized in managing one&apos;s own time and the time of others.</obo:IAO_0000115>
        <obo:IAO_0000117>Oliver He</obo:IAO_0000117>
        <obo:IAO_0000117>Sam Smith</obo:IAO_0000117>
        <obo:IAO_0000119>https://www.onetonline.org/find/descriptor/browse/2.B/2.B.2/2.B.5/2.B.1/2.B.4/2.B.3</obo:IAO_0000119>
        <obo:OCCO_00000008>2.B.5.a</obo:OCCO_00000008>
        <rdfs:label>time management</rdfs:label>
    </owl:Class>
    


    <!-- http://purl.obolibrary.org/obo/OCCO_00000053 -->

    <owl:Class rdf:about="http://purl.obolibrary.org/obo/OCCO_00000053">
        <rdfs:subClassOf rdf:resource="http://purl.obolibrary.org/obo/OCCO_00000003"/>
        <obo:IAO_0000115>A skill realized in determining causes of operating errors and deciding what to do about it.</obo:IAO_0000115>
        <obo:IAO_0000117>Oliver He</obo:IAO_0000117>
        <obo:IAO_0000117>Sam Smith</obo:IAO_0000117>
        <obo:IAO_0000119>https://www.onetonline.org/find/descriptor/browse/2.B/2.B.2/2.B.5/2.B.1/2.B.4/2.B.3</obo:IAO_0000119>
        <obo:OCCO_00000008>2.B.3.k</obo:OCCO_00000008>
        <rdfs:label>troubleshooting</rdfs:label>
    </owl:Class>
    


    <!-- http://purl.obolibrary.org/obo/OCCO_00000054 -->

    <owl:Class rdf:about="http://purl.obolibrary.org/obo/OCCO_00000054">
        <rdfs:subClassOf rdf:resource="http://purl.obolibrary.org/obo/OCCO_00000003"/>
        <obo:IAO_0000115>A skill realized in communicating effectively in writing as appropriate for the needs of the audience.</obo:IAO_0000115>
        <obo:IAO_0000117>Oliver He</obo:IAO_0000117>
        <obo:IAO_0000117>Sam Smith</obo:IAO_0000117>
        <obo:IAO_0000119>https://www.onetonline.org/find/descriptor/browse/2.A/2.A.1/2.A.2</obo:IAO_0000119>
        <obo:OCCO_00000008>2.A.1.c</obo:OCCO_00000008>
        <rdfs:label>writing</rdfs:label>
    </owl:Class>
</rdf:RDF>



<!-- Generated by the OWL API (version 4.5.26) https://github.com/owlcs/owlapi -->

